specs/Spec.Agile.Hash.fsti
@@ -59,19 +59,27 @@ val update (a:md_alg): update_t a
 let update_multi_pre
   (a:hash_alg)
   (hash:words_state a)
-  (blocks:bytes_blocks a)
+  (blocks:bytes)
 =
   match a with
-  | Blake2B | Blake2S -> (S.length blocks + snd hash) `less_than_max_input_length` a
+  | Blake2B | Blake2S ->
+      let _, prev = hash <: (words_state' a & nat) in
+      (S.length blocks + prev) `less_than_max_input_length` a
   | _ -> true
 
+(* Agile multi-block processing function shown to obey the hash laws. *)
 val update_multi
   (a:hash_alg)
   (hash:words_state a)
   (blocks:bytes_blocks a):
   Pure (words_state a)
     (requires update_multi_pre a hash blocks)
-    (ensures fun _ -> True)
+    (ensures fun hash' ->
+      if is_blake a then
+        snd (hash' <: words_state' a & nat) ==
+        snd (hash <: words_state' a & nat) + S.length blocks
+      else
+        True)
 
 val hash (a:hash_alg) (input:bytes{S.length input `less_than_max_input_length` a}):
   Tot (Lib.ByteSequence.lbytes (hash_length a))
