specs/Spec.Hash.PadFinish.fst
@@ -50,26 +50,24 @@ let pad (a:md_alg)
 
 (* Unflatten the hash from the sequence of words to bytes up to the correct size *)
 let finish_md (a:md_alg) (hashw:words_state a): Tot (lbytes (hash_length a)) =
-  let hashw, extra = hashw in
   let hash_final_w = S.slice hashw 0 (hash_word_length a) in
   bytes_of_words a #(hash_word_length a) hash_final_w
 
-let finish_blake (a:blake_alg) (hashw:words_state a): Tot (lbytes (hash_length a)) =
+let finish_blake (a:blake_alg) (hash:words_state' a): Tot (lbytes (hash_length a)) =
   let alg = to_blake_alg a in
-  Spec.Blake2.blake2_finish alg (fst hashw) (Spec.Blake2.max_output alg)
+  Spec.Blake2.blake2_finish alg hash (Spec.Blake2.max_output alg)
 
 let finish_sha3 (a: sha3_alg) (s: words_state a): Tot (lbytes (hash_length a)) =
   match a with
   | SHA3_256 ->
       let rateInBytes = 1088 / 8 in
       let outputByteLen = 32 in
-      let s, _ = s in
       Spec.SHA3.squeeze s rateInBytes outputByteLen
 
 (* Note that the ``extra_state`` in the ``words_state`` parameter is useless -
  * we use this fact pervasively in the proofs and some definitions by providing
  * dummy extra-states when we don't manipulate "full" words states *)
-let finish (a:hash_alg) (hashw:words_state a): Tot (lbytes (hash_length a)) =
+let finish (a:hash_alg) (hashw:words_state' a): Tot (lbytes (hash_length a)) =
   if is_blake a then
     finish_blake a hashw
   else if is_sha3 a then
