specs/lemmas/Spec.Blake2.Incremental.fst
@@ -1,5 +1,17 @@
 module Spec.Blake2.Incremental
 
+module S = FStar.Seq
 
-// TODO: move proof currently located in Hacl.Streaming.Blake2
-let blake2_is_hash_incremental _ _ = admit ()
+open Spec.Agile.Hash
+open Spec.Hash.Definitions
+open Spec.Hash.Incremental.Definitions
+open Spec.Hash.PadFinish
+open Spec.Hash.Lemmas
+open FStar.Mul
+
+friend Spec.Agile.Hash
+
+// TODO: move or reuse currently located in Hacl.Streaming.Blake2
+let blake2_is_hash_incremental a input =
+  admit ()
+
