specs/lemmas/Spec.Blake2.Incremental.fsti
@@ -1,8 +1,6 @@
 module Spec.Blake2.Incremental
 
 module S = FStar.Seq
-module Blake2 = Spec.Blake2
-module Loops = Lib.LoopCombinators
 
 open Spec.Agile.Hash
 open Spec.Hash.Definitions
@@ -15,5 +13,5 @@ val blake2_is_hash_incremental
   (a : blake_alg)
   (input : bytes {S.length input `less_than_max_input_length` a}) :
   Lemma (
-    S.equal (Blake2.blake2 (to_blake_alg a) input 0 Seq.empty (Spec.Blake2.max_output (to_blake_alg a)))
+    S.equal (Spec.Blake2.blake2 (to_blake_alg a) input 0 Seq.empty (Spec.Blake2.max_output (to_blake_alg a)))
             (hash_incremental a input))
